chore: lean refactor
commit-id:e99d587d

lean/privacy/channels/channels.lean
@@ -10,55 +10,159 @@ def channel_exists (crypto: Crypto) (m: Memory) (c: ℕ) : Prop :=
   ∃ (addralice addrbob Kbob: ℕ),
     m .ChannelHashes [crypto.hash [c, addralice, addrbob, Kbob]] ≠ 0
 
--- CreateChannel action → Kbob has a corresponding private key.
-theorem exists_private_key
-    {crypto: Crypto} {inp: CreateChannelInput} {rm: ReachableMemory crypto}
-    (success: (create_channel crypto inp rm |> process_action crypto rm).success) :
-    ∃ kbob: crypto.PrivateKeys,
-      inp.Kbob = crypto.priv_to_pub kbob ∧
-      rm.m .PublicKeys [inp.addrbob] = inp.Kbob := by
-  let info := create_channel_info crypto inp rm success
-  have bob_registered := info.bob_registered
-  rw [←info.h_Kbob] at bob_registered
+structure ChannelImplies
+    {crypto: Crypto} (rm: ReachableMemory crypto) (inp: CreateChannelInput) where
+  h_action: .CreateChannel inp ∈ rm.actions
+  success: ∃ rm₀: ReachableMemory crypto, ∃ success, rm.extends (rm₀.add (.CreateChannel inp) success)
+  kbob: crypto.PrivateKeys
+  h_Kbob: inp.Kbob = crypto.priv_to_pub kbob
+  alice_registered: RegisterImplies rm ⟨inp.addralice, inp.kalice⟩
+  bob_registered: RegisterImplies rm ⟨inp.addrbob, kbob⟩
+  channel_hashes: rm.m .ChannelHashes [crypto.hash [inp.c crypto, inp.addralice, inp.addrbob, inp.Kbob]] ≠ 0
+  j: ℕ
+  h_j_lt: j < rm.m .ChannelsJ [inp.addrbob]
+  channel_enc: rm.m .Channels [inp.addrbob, j] = inp.enc crypto
 
-  have ⟨kalice, h⟩ := public_keys bob_registered
-  exact ⟨kalice, by rw [←info.h_Kbob, h], by rw [info.h_Kbob]⟩
+abbrev ChannelImplies.c
+    {crypto: Crypto} {rm: ReachableMemory crypto} {inp: CreateChannelInput}
+    (_: ChannelImplies rm inp) : ℕ :=
+  inp.c crypto
+
+theorem ChannelImplies.h_channel_exists
+    {crypto: Crypto} {rm: ReachableMemory crypto} {inp: CreateChannelInput}
+    (channel_imp: ChannelImplies rm inp) :
+    channel_exists crypto rm (inp.c crypto) :=
+  ⟨inp.addralice, inp.addrbob, inp.Kbob, by simp [channel_imp.channel_hashes]⟩
+
+theorem ChannelImplies.next
+    {crypto: Crypto} {rm: ReachableMemory crypto} {inp: CreateChannelInput}
+    {action: Action} (success: (run_action crypto action rm.m).success)
+    (channel_imp: ChannelImplies rm inp) :
+    Nonempty (ChannelImplies (rm.add action success) inp) := by
+  have ⟨rm₀, h_success, ℓ, h_extends⟩ := channel_imp.success
+  unfold ReachableMemory.add at h_extends
+  refine ⟨{
+    h_action := by simp [channel_imp.h_action],
+    success := ⟨rm₀, h_success, action::ℓ, by simp [h_extends]⟩,
+    kbob := channel_imp.kbob,
+    h_Kbob := channel_imp.h_Kbob,
+    alice_registered := channel_imp.alice_registered.next success,
+    bob_registered := channel_imp.bob_registered.next success,
+    channel_hashes := ?_
+    h_j_lt := ?_,
+    j := channel_imp.j,
+    channel_enc := ?_
+  }⟩
+
+  · cases action
+    case CreateChannel inp' =>
+      let info := create_channel_info crypto inp' rm success
+      rw [rm.add_m, run_action, ←info.h_m']
+      by_cases h_is_same: inp.channel_hash crypto = inp'.channel_hash crypto
+      case pos =>
+        rw [←CreateChannelInput.channel_hash, h_is_same]
+        simp [info.memory_diff₂]
+      case neg =>
+        rw [info.no_change _ _ (by simp; simp [h_is_same])]
+        exact channel_imp.channel_hashes
+    all_goals exact channel_imp.channel_hashes
+
+  · cases action
+    case CreateChannel inp' =>
+      let info := create_channel_info crypto inp' rm success
+      rw [rm.add_m, run_action, ←info.h_m']
+      by_cases h_addrbob: inp.addrbob = inp'.addrbob
+      case pos =>
+        rw [h_addrbob, info.memory_diff₀]
+        have := h_addrbob ▸ channel_imp.h_j_lt
+        omega
+      case neg =>
+        rw [info.no_change _ _ (by simp [h_addrbob])]
+        exact channel_imp.h_j_lt
+
+    all_goals exact channel_imp.h_j_lt
+
+  · cases action
+    case CreateChannel inp' =>
+      let info := create_channel_info crypto inp' rm success
+      rw [rm.add_m, run_action, ←info.h_m']
+      have h: inp.addrbob = inp'.addrbob → ¬channel_imp.j = info.j := by
+        intro h_addrbob
+        by_contra h'
+        have := channel_imp.h_j_lt
+        simp [h_addrbob, info.h_j, h'] at this
+      rw [info.no_change _ _ (by simpa)]
+      exact channel_imp.channel_enc
+
+    all_goals exact channel_imp.channel_enc
+
+theorem ChannelImplies.from_action
+    {crypto: Crypto} {rm: ReachableMemory crypto} {inp: CreateChannelInput}
+    (h: .CreateChannel inp ∈ rm.actions) :
+    Nonempty (ChannelImplies rm inp) := by
+  revert rm
+  apply ReachableMemory.induction
+  case inv₀ => simp
+
+  intro action rm ih success h
+  cases h
+  case head =>
+    let info := create_channel_info crypto inp rm success
+    have ⟨kbob, res_bob⟩ := RegisterImplies.from_public_key (info.h_Kbob ▸ info.bob_registered)
+    have : rm.m MemoryType.PublicKeys [inp.addralice] ≠ 0 := by
+      rw [info.alice_registered]
+      exact crypto.zero_not_public_key ⟨inp.kalice, info.kalice_valid⟩
+    have ⟨kalice, res_alice⟩ := RegisterImplies.from_public_key this
+    have h_kalice : kalice = inp.kalice := by
+      apply crypto.priv_to_pub_inj (by simp) info.kalice_valid
+      rw [←info.alice_registered, res_alice.public_key]
+
+    exact ⟨{
+      h_action := by simp
+      success := ⟨rm, success, [], by simp⟩,
+      kbob := kbob
+      h_Kbob := by rw [←info.h_Kbob, res_bob.public_key]
+      alice_registered := h_kalice ▸ res_alice.next success
+      bob_registered := res_bob.next success
+      channel_hashes := by rw [rm.add_m, run_action, ←info.h_m', info.memory_diff₂]; simp
+      j := info.j
+      h_j_lt := by rw [rm.add_m, run_action, ←info.h_m', info.memory_diff₀, info.h_j]; simp
+      channel_enc := by rw [rm.add_m, run_action, ←info.h_m', info.memory_diff₁]
+    }⟩
+
+  case tail h =>
+    have ⟨ih⟩ := ih h
+    exact ih.next success
 
 -- Channel hash entry implies c is a valid channel id and Kbob is a valid public key.
-theorem channel_exists_implies_hash
-    {crypto: Crypto} {c addralice addrbob Kbob: ℕ} :
-    ∀ {rm: ReachableMemory crypto},
-    rm.m .ChannelHashes [crypto.hash [c, addralice, addrbob, Kbob]] ≠ 0 →
-    (∃ kalice: crypto.PrivateKeys,
-      c = crypto.hash [addralice, kalice, addrbob, Kbob] ∧
-      rm.m .PublicKeys [addralice] = crypto.priv_to_pub kalice
-    ) ∧
-    (∃ kbob: crypto.PrivateKeys,
-      Kbob = crypto.priv_to_pub kbob ∧
-      rm.m .PublicKeys [addrbob] = Kbob
-    ) := by
+theorem ChannelImplies.from_channel_hashes
+    {crypto: Crypto} {rm: ReachableMemory crypto} {c addralice addrbob Kbob: ℕ}
+    (h: rm.m .ChannelHashes [crypto.hash [c, addralice, addrbob, Kbob]] ≠ 0) :
+    ∃ (kalice s r: ℕ) (res: ChannelImplies rm ⟨addralice, kalice, addrbob, Kbob, s, r⟩),
+    res.c = c := by
+  suffices h' : ∃ kalice s r: ℕ,
+      (.CreateChannel ⟨addralice, kalice, addrbob, Kbob, s, r⟩) ∈ rm.actions ∧
+      c = crypto.hash [addralice, kalice, addrbob, Kbob] from by
+    obtain ⟨kalice, s, r, h'⟩ := h'
+    have ⟨res⟩ := ChannelImplies.from_action h'.1
+    use kalice, s, r, res
+    simp [ChannelImplies.c, CreateChannelInput.c, h'.2]
+
+  revert rm
   apply ReachableMemory.induction
   case inv₀ => intro h; trivial
 
-  intro action rm ih success
+  intro action rm ih success h
   cases action
   case CreateChannel inp =>
     let info := create_channel_info crypto inp rm success
-    dsimp only [ReachableMemory.add, ReachableMemory.m]
-    rw [run_all_cons₁, run_action, ←info.h_m']
-    intro h'
+    dsimp only [ReachableMemory.add, ReachableMemory.m] at h
+    rw [run_all_cons₁, run_action, ←info.h_m'] at h
 
     by_cases h_is_same: c = inp.c crypto ∧ addralice = inp.addralice ∧ addrbob = inp.addrbob ∧ Kbob = inp.Kbob
     case pos =>
       simp only [h_is_same]
-      constructor
-      · use ⟨inp.kalice, info.kalice_valid⟩
-        constructor
-        · trivial
-        · rw [info.no_change _ _ (by simp)]
-          exact info.alice_registered
-      · conv => rhs; intro kbob; rw [info.no_change _ _ (by simp)]
-        exact exists_private_key success
+      use inp.kalice, inp.s, inp.r, by simp
     case neg =>
       rw [info.no_change _ _  (by
         simp only [ne_eq, Prod.mk.injEq, reduceCtorEq, List.cons.injEq, and_true, false_and,
@@ -67,83 +171,40 @@ theorem channel_exists_implies_hash
         apply crypto.h_hash at h'
         repeat injection h' with _ h'
         simp [*] at h_is_same
-      )] at h'
-      conv => rhs; rhs; intro m'; rw [info.no_change _ _ (by simp)]
-      conv => lhs; rhs; intro m'; rw [info.no_change _ _ (by simp)]
-      exact ih h'
+      )] at h
+      have ⟨kalice, s, r, ⟨h_actions, h_c⟩⟩ := ih h
+      use kalice, s, r, by simp [h_actions]
 
-  case Register inp =>
-    intro h
-    let info := register_info crypto inp rm success
-    rw [rm.add_m, run_action, ←info.h_m']
+  all_goals
+    have ⟨kalice, s, r, ⟨h_actions, h_c⟩⟩ := ih h
+    use kalice, s, r, by simp [h_actions]
 
-    have ⟨⟨kalice, h₀, h₁⟩, ⟨kbob, h₂, h₃⟩⟩ := ih h
-    refine ⟨⟨kalice, h₀, ?_⟩, ⟨kbob, h₂, ?_⟩⟩
-    · by_cases h_is_same: addralice = inp.addralice
-      case pos =>
-        rw [h_is_same, info.alice_was_not_registered] at h₁
-        have := crypto.zero_not_public_key kalice
-        simp [h₁] at this
-      case neg => rwa [info.no_change _ _ (by simp [h_is_same])]
-    · by_cases h_is_same: addrbob = inp.addralice
-      case pos =>
-        rw [h_is_same, info.alice_was_not_registered] at h₃
-        have := crypto.zero_not_public_key kbob
-        simp [h₃, h₂] at this
-      case neg => rwa [info.no_change _ _ (by simp [h_is_same])]
+theorem ChannelImplies.same_c
+    {crypto: Crypto} {rm: ReachableMemory crypto} {inp: CreateChannelInput}
+    (channel_imp: ChannelImplies rm inp)
+    {addralice kalice addrbob Kbob: ℕ}
+    (h: channel_imp.c = crypto.hash [addralice, kalice, addrbob, Kbob]) :
+    addralice = inp.addralice ∧ kalice = inp.kalice ∧ addrbob = inp.addrbob ∧ Kbob = inp.Kbob := by
+  apply crypto.h_hash at h; injections; simp [*]
 
-  all_goals exact ih
+theorem ChannelImplies.same_c_priv
+    {crypto: Crypto} {rm: ReachableMemory crypto} {inp: CreateChannelInput}
+    (channel_imp: ChannelImplies rm inp)
+    {addralice kalice addrbob: ℕ}
+    {kbob: crypto.PrivateKeys}
+    (h: channel_imp.c = crypto.hash [addralice, kalice, addrbob, crypto.priv_to_pub kbob]) :
+    addralice = inp.addralice ∧ kalice = inp.kalice ∧ addrbob = inp.addrbob ∧ kbob = channel_imp.kbob := by
+  have := channel_imp.same_c h
+  simp only [*, true_and]
+  apply Subtype.coe_inj.1
+  apply crypto.priv_to_pub_inj (by simp) (by simp)
+  simp [this.2.2.2, channel_imp.h_Kbob]
 
-theorem channel_exists_iff_CreateChannel {crypto: Crypto} {rm: ReachableMemory crypto} {c: ℕ} :
-    channel_exists crypto rm c ↔
-    (∃ inp: CreateChannelInput, .CreateChannel inp ∈ rm.actions ∧ inp.c crypto = c) := by
-  revert rm
-  apply ReachableMemory.induction
-  case inv₀ =>
-    constructor
-    · intro h
-      have ⟨addralice, addrbob, Kbob, h⟩ := h
-      simp [ReachableMemory.m] at h
-    · intro h; simp at h
-
-  intro action rm ih success
-  cases action
-  case CreateChannel inp' =>
-    let info := create_channel_info crypto inp' rm success
-    rw [ReachableMemory.add_m, run_action, ←info.h_m']
-    simp only [channel_exists]
-
-    by_cases h_is_same: c = inp'.c crypto
-    case pos =>
-      constructor
-      · intro h
-        obtain ⟨addralice, addrbob, Kbob, h⟩ := h
-        exact ⟨inp', by simp [ReachableMemory.add], by simp [h_is_same]⟩
-      · intro h
-        use inp'.addralice, inp'.addrbob, inp'.Kbob
-        simp [h_is_same, info.memory_diff₂]
-    case neg =>
-      conv in _ ≠ 0 => rw [info.no_change _ _ (by
-        have : crypto.hash [c, addralice, addrbob, Kbob] ≠ inp'.channel_hash crypto := by
-          by_contra h'; apply crypto.h_hash at h'; injections; contradiction
-        simp [this]
-      )]
-      rw [ReachableMemory.add]
-
-      conv in _ ∈ _ => rw [List.mem_cons, Action.CreateChannel.injEq]
-      rw [←channel_exists, ih]
-
-      constructor
-      · intro h
-        have ⟨inp, h₀, h₁⟩ := h
-        exact ⟨inp, Or.inr h₀, h₁⟩
-      · intro h
-        obtain ⟨inp, h₀, h₁⟩ := h
-        cases h₀
-        case inl h₀ =>
-          rw [←h₁, h₀] at h_is_same
-          contradiction
-        case inr h₀ =>
-          exact ⟨inp, h₀, h₁⟩
-
-  all_goals simpa [ReachableMemory.add]
+theorem ChannelImplies.from_channel_exists
+    {crypto: Crypto} {rm: ReachableMemory crypto} {c: ℕ}
+    (h: channel_exists crypto rm c) :
+    ∃ (inp: CreateChannelInput) (channel_imp: ChannelImplies rm inp),
+    channel_imp.c = c := by
+  replace ⟨addralice, addrbob, Kbob, h⟩ := h
+  have ⟨kalice, s, r, ⟨channel_imp, h_c⟩⟩ := ChannelImplies.from_channel_hashes h
+  use ⟨addralice, kalice, addrbob, Kbob, s, r⟩, channel_imp
