lean/privacy/registration/registration.lean
@@ -27,13 +27,72 @@ theorem public_keys {crypto: Crypto} {addralice: ℕ} :
       exact h
   repeat intro h success; exact h
 
-theorem public_key_implies {crypto: Crypto} {rm: ReachableMemory crypto} {addralice: ℕ}
+structure RegisterImplies
+    {crypto: Crypto} (rm: ReachableMemory crypto) (inp: RegisterInput) where
+  h_action: .Register inp ∈ rm.actions
+  public_key: rm.m .PublicKeys [inp.addralice] = crypto.priv_to_pub inp.kalice
+  h_kalice: inp.kalice ∈ crypto.PrivateKeys
+
+theorem RegisterImplies.from_action
+    {crypto: Crypto} {rm: ReachableMemory crypto} {inp: RegisterInput}
+    (h: .Register inp ∈ rm.actions) :
+    RegisterImplies rm inp := by
+  revert rm
+  apply ReachableMemory.induction
+  case inv₀ => simp
+
+  intro action rm ih success h
+  rw [ReachableMemory.add] at h
+
+  cases h
+  case head =>
+    let info := register_info crypto inp _ success
+
+    exact {
+      h_action := by simp,
+      public_key := by
+        rw [rm.add_m, run_action, ←info.h_m']
+        rw [info.memory_diff₀]
+      h_kalice := info.kalice_private_key
+    }
+
+  case tail h =>
+    have ih := ih h
+
+    cases action
+    case Register inp' =>
+      let info := register_info crypto inp' _ success
+
+      have h_addralice : inp.addralice ≠ inp'.addralice := by
+        by_contra h₀
+        exact crypto.zero_not_public_key ⟨inp.kalice, ih.h_kalice⟩ (Eq.symm (info.alice_was_not_registered ▸ h₀ ▸ ih.public_key))
+
+      exact {
+        h_action := by simp [ih.h_action],
+        public_key := by
+          rw [rm.add_m, run_action, ←info.h_m']
+          rw [info.no_change _ _ (by simp [h_addralice])]
+          exact ih.public_key
+        h_kalice := ih.h_kalice
+      }
+
+    all_goals
+      refine ⟨?_, ?_, ?_⟩
+      · simp [ih.h_action]
+      · exact ih.public_key
+      · exact ih.h_kalice
+
+theorem RegisterImplies.next
+    {crypto: Crypto} {rm: ReachableMemory crypto} {inp: RegisterInput}
+    {action: Action} (success: (run_action crypto action rm.m).success)
+    (h: RegisterImplies rm inp) :
+    RegisterImplies (rm.add action success) inp :=
+  RegisterImplies.from_action (by simp [h.h_action])
+
+theorem RegisterImplies.from_public_key {crypto: Crypto} {rm: ReachableMemory crypto} {addralice: ℕ}
     (h: rm.m .PublicKeys [addralice] ≠ 0) :
-    ∃ inp: RegisterInput,
-      .Register inp ∈ rm.actions ∧
-      inp.addralice = addralice ∧
-      rm.m .PublicKeys [addralice] = crypto.priv_to_pub inp.kalice ∧
-      inp.kalice ∈ crypto.PrivateKeys := by
+    ∃ kalice: crypto.PrivateKeys,
+      RegisterImplies rm ⟨addralice, kalice⟩ := by
   revert rm
   apply ReachableMemory.induction
   case inv₀ => simp [ReachableMemory.m]
@@ -42,17 +101,19 @@ theorem public_key_implies {crypto: Crypto} {rm: ReachableMemory crypto} {addral
   cases action
   case Register inp =>
     let info := register_info crypto inp rm success
-    rw [rm.add_m, run_action, ←info.h_m'] at ⊢ h
+
     by_cases h_is_same: addralice = inp.addralice
     case pos =>
-      use inp
-      simp only [h_is_same, info.memory_diff₀, info.kalice_private_key]
+      use ⟨inp.kalice, info.kalice_private_key⟩
+      simp only [h_is_same]
+      apply RegisterImplies.from_action
       simp
     case neg =>
-      rw [info.no_change _ _ (by simp [h_is_same])] at ⊢ h
-      have ⟨inp, h₀, h₁⟩ := ih h
-      exact ⟨inp, by simp [ReachableMemory.add, h₀], h₁⟩
+      rw [rm.add_m, run_action, ←info.h_m'] at h
+      rw [info.no_change _ _ (by simp [h_is_same])] at h
+      have ⟨kalice, res⟩ := ih h
+      exact ⟨kalice, res.next success⟩
 
   all_goals
-    have ⟨inp, h₀, h₁⟩ := ih h
-    exact ⟨inp, by simp [ReachableMemory.add, h₀], h₁⟩
+    have ⟨kalice, res⟩ := ih h
+    exact ⟨kalice, res.next success⟩
