lean/privacy/notes/note_implies.lean
@@ -1,0 +1,157 @@
+import privacy.actions
+import privacy.subchannels.subchannels
+import privacy.notes.notes
+import privacy.utils
+
+structure NoteImplies {crypto: Crypto} (rm: ReachableMemory crypto) (inp: CreateNoteInput) where
+  h_action: .CreateNote inp ∈ rm.actions
+  h_i₀: inp.i₀ < crypto.MAX_I₀
+  subchannel: SubchannelImplies rm (inp.c crypto) inp.addralice inp.addrbob inp.Kbob inp.token
+  h_note_exists: note_exists rm (inp.note_id crypto)
+  h_open_note: inp.r = 1 → rm.m .OpenNoteToken [inp.note_id crypto] = inp.token
+  h_r: (crypto.unpack (rm.m .Notes [inp.note_id crypto, 0])).1 = inp.r
+
+theorem NoteImplies.h_kalice
+    {crypto: Crypto} {rm: ReachableMemory crypto} {inp: CreateNoteInput}
+    (note_imp: NoteImplies rm inp) :
+    inp.kalice = note_imp.subchannel.kalice := by
+  simp [note_imp.subchannel.channel.same_c (Eq.symm note_imp.subchannel.h_c)]
+
+theorem NoteImplies.h_Kbob
+    {crypto: Crypto} {rm: ReachableMemory crypto} {inp: CreateNoteInput}
+    (note_imp: NoteImplies rm inp) :
+    crypto.priv_to_pub note_imp.subchannel.channel.kbob = inp.Kbob := by
+  rw [←note_imp.subchannel.channel.h_Kbob]
+
+theorem NoteImplies.next
+    {crypto: Crypto} {rm: ReachableMemory crypto} {inp: CreateNoteInput}
+    {action: Action} (success: (run_action crypto action rm.m).success)
+    (note_imp: NoteImplies rm inp) :
+    Nonempty (NoteImplies (rm.add action success) inp) := by
+  cases action
+  case CreateNote inp' =>
+    let info := create_note_info crypto inp' rm success
+    have h_note_id : inp.note_id crypto ≠ inp'.note_id crypto :=
+        λ h_note_id ↦ absurd (h_note_id ▸ info.old_value_was_zero) note_imp.h_note_exists
+
+    constructor; constructor
+    case h_action => simp [note_imp.h_action]
+    case h_i₀ => exact note_imp.h_i₀
+    case subchannel => exact Nonempty.some (note_imp.subchannel.next success)
+    case h_note_exists => exact note_exists_monotone success note_imp.h_note_exists
+
+    all_goals
+      rw [ReachableMemory.add_m, run_action, ←info.h_m']
+      rw [info.no_change _ _ (by simp [h_note_id]) (by simp [h_note_id])]
+
+    case h_open_note => exact note_imp.h_open_note
+    case h_r => exact note_imp.h_r
+
+  case OpenDeposit inp' =>
+    let info := open_deposit_info crypto inp' rm success
+
+    refine ⟨{
+      h_action := by simp [note_imp.h_action],
+      h_i₀ := note_imp.h_i₀,
+      subchannel := Nonempty.some (note_imp.subchannel.next success),
+      h_note_exists := note_exists_monotone success note_imp.h_note_exists,
+      h_open_note := note_imp.h_open_note,
+      h_r := ?_,
+    }⟩
+
+    have h_r := note_imp.h_r
+    rw [ReachableMemory.add_m, run_action, ←info.h_m']
+
+    by_cases h_is_same: inp.note_id crypto = inp'.note_id
+    case pos =>
+      rw [h_is_same, info.old_value] at h_r
+      rw [h_is_same, info.memory_diff₀, ←h_r, crypto.unpack_pack, crypto.unpack_pack]
+    case neg =>
+      rw [info.no_change _ _ (by simp [h_is_same])]
+      exact h_r
+
+  all_goals exact ⟨{
+    h_action := by simp [note_imp.h_action],
+    h_i₀ := note_imp.h_i₀,
+    subchannel := Nonempty.some (note_imp.subchannel.next success),
+    h_note_exists := note_exists_monotone success note_imp.h_note_exists,
+    h_open_note := note_imp.h_open_note,
+    h_r := note_imp.h_r,
+  }⟩
+
+theorem NoteImplies.from_action
+    {crypto: Crypto} {rm: ReachableMemory crypto} {inp: CreateNoteInput}
+    (h: .CreateNote inp ∈ rm.actions) :
+    Nonempty (NoteImplies rm inp) := by
+  revert rm
+  apply ReachableMemory.induction
+  case inv₀ => intro h; contradiction
+
+  intro action rm ih success h
+  cases h
+  case head =>
+    let info := create_note_info crypto inp rm success
+    have ⟨addralice, ⟨subchannel_imp⟩⟩ := SubchannelImplies.from_subchannel_hash_exists info.subchannel_exists
+    have h_addralice: inp.addralice = addralice := by
+      simp [subchannel_imp.channel.same_c (Eq.symm subchannel_imp.h_c)]
+
+    constructor; constructor
+
+    case h_action => simp
+    case h_i₀ => exact info.i₀_lt_MAX_I₀
+    case subchannel => rw [h_addralice]; exact Nonempty.some (subchannel_imp.next success)
+    case h_note_exists =>
+      rw [ReachableMemory.add_m, run_action, ←info.h_m', note_exists, info.memory_diff₀]
+      exact crypto.pack_nz info.r_ne_zero
+    case h_open_note =>
+      intro r_eq_one
+      rw [ReachableMemory.add_m, run_action, ←info.h_m', info.memory_diff₁]
+      simp [r_eq_one]
+    case h_r =>
+      rw [ReachableMemory.add_m, run_action, ←info.h_m', info.memory_diff₀]
+      rw [crypto.unpack_pack]
+
+  case tail h =>
+    have ⟨ih⟩ := ih h
+    exact ih.next success
+
+theorem NoteImplies.from_note_exists
+    {crypto: Crypto} {rm: ReachableMemory crypto} {note_id: ℕ}
+    (h_note_exists: note_exists rm note_id) :
+    ∃ (inp: CreateNoteInput) (_: NoteImplies rm inp), inp.note_id crypto = note_id := by
+  suffices h' : ∃ inp: CreateNoteInput, .CreateNote inp ∈ rm.actions ∧ inp.note_id crypto = note_id from by
+    obtain ⟨inp, h'⟩ := h'
+    have ⟨note_imp⟩ := NoteImplies.from_action h'.1
+    use inp, note_imp
+    simp [h'.2]
+
+  revert rm
+  apply ReachableMemory.induction
+  case inv₀ => intro h; contradiction
+
+  intro action rm ih success
+  cases action
+  case CreateNote inp =>
+    let info := create_note_info crypto inp rm success
+    by_cases h_note_id : note_id = inp.note_id crypto
+    case pos => simp [h_note_id]
+    case neg =>
+      intro h_note_exists
+      have : note_exists rm.m note_id := by
+        unfold note_exists at *
+        rw [ReachableMemory.add_m, run_action, ←info.h_m'] at h_note_exists
+        rw [info.no_change _ _ (by simp [h_note_id]) (by simp)] at h_note_exists
+        exact h_note_exists
+      obtain ⟨inp, ih₀, ih₁⟩ := ih this
+      exact ⟨inp, by simp [ih₀], ih₁⟩
+
+  case OpenDeposit inp' =>
+    rw [note_exists_open_deposit success]
+    intro h
+    obtain ⟨inp, ih₀, ih₁⟩ := ih h
+    exact ⟨inp, by simp [ih₀], ih₁⟩
+
+  all_goals
+    intro h
+    obtain ⟨inp, ih₀, ih₁⟩ := ih h
+    exact ⟨inp, by simp [ih₀], ih₁⟩
